subst-subst-distr finish

src/Pipit.Exp.Binding.Properties.fst
@@ -234,8 +234,6 @@ let lemma_subst_subst_distribute_le_XMu
     C.lemma_lift_drop_eq 'c i1;
 
     assert (C.get_index ('a :: 'c) (i1 + 1) == C.get_index 'c i1);
-    assert (subst1' (subst1' (XMu e) i1 p1) i2 p2 ==
-      XMu (subst1' (subst1' e (i1 + 1) p1') (i2 + 1) p2'));
 
     C.lemma_dropCons 'a 'c (i2 + 2);
     C.lemma_dropCons 'a (C.drop1 'c (i2 + 1)) (i1 + 1);
@@ -243,52 +241,62 @@ let lemma_subst_subst_distribute_le_XMu
     assert (C.get_index ('a :: 'c) (i2 + 2) == C.get_index ('a :: C.drop1 'c i1) (i2 + 1));
     C.lemma_dropCons 'a 'c (i2 + 1);
     C.lemma_dropCons 'a (C.drop1 'c i1) (i2 + 1);
-    // C.lemma_lift_drop_commute_le
     assert (C.drop1 ('a :: 'c) (i2 + 2) == C.lift1 (C.drop1 ('a :: C.drop1 'c i1) (i2 + 1)) (i1 + 1) (C.get_index 'c i1));
-
 
     C.lemma_drop_drop_commute 'c i1 i2;
     C.lemma_drop_get_index_lt 'c (i2 + 1) i1;
-    assert (subst1' (subst1' e (i1 + 1) p1') (i2 + 1) p2' == subst1' (subst1' e (i2 + 2) (lift1' p2' (i1 + 1) (C.get_index 'c i1))) (i1 + 1) (subst1' p1' (i2 + 1) p2'));
-    assert (subst1' (subst1' (XMu e) i1 p1) i2 p2 == XMu (subst1' (subst1' e (i1 + 1) p1') (i2 + 1) p2'));
-    assert (XMu (coerce_eq () (subst1' (subst1' e (i1 + 1) p1') (i2 + 1) p2')) == XMu #(C.drop1 (C.drop1 'c (i2 + 1)) i1) (subst1' (subst1' e (i2 + 2) (lift1' p2' (i1 + 1) (C.get_index 'c i1))) (i1 + 1) (subst1' p1' (i2 + 1) p2')));
-
+    assert (subst1' (subst1' (XMu e) i1 p1) i2 p2 ==
+            XMu (subst1' (subst1' e (i1 + 1) p1') (i2 + 1) p2'));
+    assert (XMu (coerce_eq () (subst1' (subst1' e (i1 + 1) p1') (i2 + 1) p2')) ==
+            XMu #(C.drop1 (C.drop1 'c (i2 + 1)) i1) (subst1' (subst1' e (i2 + 2) (lift1' p2' (i1 + 1) (C.get_index 'c i1))) (i1 + 1) (subst1' p1' (i2 + 1) p2')));
     assert (subst1' (subst1' (XMu e) (i2 + 1) (lift1' p2 i1 (C.get_index 'c i1))) i1 (subst1' p1 i2 p2) ==
             XMu (subst1' (subst1' e (i2 + 2) (lift1 (lift1' p2 i1 (C.get_index 'c i1)) 'a)) (i1 + 1) (lift1 (subst1' p1 i2 p2) 'a)));
-
-    assert (subst1' (subst1' (XMu e) i1 p1) i2 p2 == subst1' (subst1' (XMu e) (i2 + 1) (lift1' p2 i1 (C.get_index 'c i1))) i1 (subst1' p1 i2 p2));
+    assert (subst1' (subst1' (XMu e) i1 p1) i2 p2 ==
+            subst1' (subst1' (XMu e) (i2 + 1) (lift1' p2 i1 (C.get_index 'c i1))) i1 (subst1' p1 i2 p2));
 
     ()
-
-// let i = ()
-//     assert_norm (subst1' (subst1' (XMu e) (i2 + 1) (lift1' p2 i1 (C.get_index 'c i1))) i1 (subst1' p1 i2 p2) ==
-//       subst1' (XMu (subst1' e ((i2 + 1) + 1) (lift1 (lift1' p2 i1 (C.get_index 'c i1)) 'a))) i1 (subst1' p1 i2 p2) ==
-//       XMu (subst1' (subst1' e ((i2 + 1) + 1) (lift1 (lift1' p2 i1 (C.get_index 'c i1)) 'a)) (i1 + 1) (lift1 (subst1' p1 i2 p2) 'a))
-//       );
 
 private
 let lemma_subst_subst_distribute_le_XLet
   (e1: exp 'c 'b) (e2: exp ('b :: 'c) 'a) (i1: C.index { C.has_index 'c i1 }) (i2: C.index { i1 <= i2 /\ i2 < List.Tot.length 'c - 1 }) (p1: exp (C.drop1 'c i1) (C.get_index 'c i1)) (p2: exp (C.drop1 (C.drop1 'c i1) i2) (C.get_index (C.drop1 'c i1) i2)):
   Lemma
     (requires (lemma_subst_subst_distribute_le_def e1 i1 i2 p1 p2 /\
-               lemma_subst_subst_distribute_le_def e2 (i1 + 1) (i2 + 1) (_lift_of_drop i1 p1 'b) (_lift_of_drop i2 p2 'b)))
+               lemma_subst_subst_distribute_le_def e2 (i1 + 1) (i2 + 1) (_lift_of_drop i1 p1 'b) (coerce_eq () (_lift_of_drop i2 p2 'b))))
     (ensures (lemma_subst_subst_distribute_le_def (XLet 'b e1 e2) i1 i2 p1 p2)) =
-    admit ()
-//   | XLet b e1 e2 ->
-//   //   lemma_lift_lift_commute p i2 0 t2 b;
-//   //   let p' = _lift_of_drop i1 p b in
+    let p1' = _lift_of_drop i1 p1 'b in
+    let p2' = _lift_of_drop i2 p2 'b in
+    lemma_lift_lift_commute p2 i1 0 (C.get_index 'c i1) 'b;
+    lemma_lift_subst_distribute_le p1 i2 0 'b p2;
 
-//   //   C.lemma_lift_get_index_gt 'c i1 0 b;
-//   //   C.lemma_lift_get_index_gt (b :: 'c) (i1 + 1) (i2 + 1) t2;
+    C.lemma_lift_drop_commute_le (C.drop1 'c i1) i2 i1 (C.get_index 'c i1);
+    C.lemma_lift_drop_eq 'c i1;
 
-//   //   C.lemma_lift_drop_commute_le 'c i1 i2 t2;
+    assert (C.get_index ('b :: 'c) (i1 + 1) == C.get_index 'c i1);
 
-//   //   lemma_subst_subst_distribute_le e1 i1 i2 t2 p;
-//   //   lemma_subst_subst_distribute_le e2 (i1 + 1) (i2 + 1) t2 p';
+    C.lemma_dropCons 'b 'c (i2 + 2);
+    C.lemma_dropCons 'b (C.drop1 'c (i2 + 1)) (i1 + 1);
+    assert ('b :: C.drop1 (C.drop1 'c (i2 + 1)) i1 == C.drop1 (C.drop1 ('b :: 'c) (i2 + 2)) (i1 + 1));
+    assert (C.get_index ('b :: 'c) (i2 + 2) == C.get_index ('b :: C.drop1 'c i1) (i2 + 1));
+    C.lemma_dropCons 'b 'c (i2 + 1);
+    C.lemma_dropCons 'b (C.drop1 'c i1) (i2 + 1);
+    assert (C.drop1 ('b :: 'c) (i2 + 2) == C.lift1 (C.drop1 ('b :: C.drop1 'c i1) (i2 + 1)) (i1 + 1) (C.get_index 'c i1));
 
-//   //   ()
-//     // lemma_lift_lift_commute p2 x1 0;
-//     // lift_subst_distribute_le p1 p2 x2 0
+    C.lemma_drop_drop_commute 'c i1 i2;
+    C.lemma_drop_get_index_lt 'c (i2 + 1) i1;
+
+    let e1'l = subst1' (subst1' e1 i1 p1) i2 p2 in
+    let e2'l = subst1' (subst1' e2 (i1 + 1) p1') (i2 + 1) p2' in
+
+    assert (subst1' (subst1' (XLet 'b e1 e2) i1 p1) i2 p2 ==
+            XLet 'b e1'l e2'l);
+    assert (XLet 'b e1'l e2'l ==
+            XLet #(C.drop1 (C.drop1 'c (i2 + 1)) i1) 'b e1'l (subst1' (subst1' e2 (i2 + 2) (lift1' p2' (i1 + 1) (C.get_index 'c i1))) (i1 + 1) (subst1' p1' (i2 + 1) p2')));
+    assert (subst1' (subst1' (XLet 'b e1 e2) (i2 + 1) (lift1' p2 i1 (C.get_index 'c i1))) i1 (subst1' p1 i2 p2) ==
+            XLet 'b (subst1' (subst1' e1 (i2 + 1) (lift1' p2 i1 (C.get_index 'c i1))) i1 (subst1' p1 i2 p2)) (subst1' (subst1' e2 (i2 + 2) (lift1 (lift1' p2 i1 (C.get_index 'c i1)) 'b)) (i1 + 1) (lift1 (subst1' p1 i2 p2) 'b)));
+    assert (subst1' (subst1' (XLet 'b e1 e2) i1 p1) i2 p2 ==
+            subst1' (subst1' (XLet 'b e1 e2) (i2 + 1) (lift1' p2 i1 (C.get_index 'c i1))) i1 (subst1' p1 i2 p2));
+
+    ()
 
 
 let rec lemma_subst_subst_distribute_le (e: exp 'c 'a) (i1: C.index { C.has_index 'c i1 }) (i2: C.index { i1 <= i2 /\ i2 < List.Tot.length 'c - 1 }) (p1: exp (C.drop1 'c i1) (C.get_index 'c i1)) (p2: exp (C.drop1 (C.drop1 'c i1) i2) (C.get_index (C.drop1 'c i1) i2)):
@@ -298,10 +306,7 @@ let rec lemma_subst_subst_distribute_le (e: exp 'c 'a) (i1: C.index { C.has_inde
     subst1' (subst1' e i1 p1) i2 p2 ==
     subst1' (subst1' e (i2 + 1) (lift1' p2 i1 (C.get_index 'c i1))) i1 (subst1' p1 i2 p2)))
     (decreases e) =
-  // C.lemma_lift_drop_commute_le (C.drop1 'c i1) i2 i1 (C.get_index 'c i1);
   C.lemma_drop_drop_commute 'c i1 i2;
-  // C.lemma_lift_drop_eq 'c i1;
-  // C.lemma_drop_get_index_gt 'c i1 i2;
   C.lemma_drop_get_index_lt 'c (i2 + 1) i1;
   match e with
   | XVal _ | XVar _ | XBVar _ -> lemma_subst_subst_distribute_le_base e i1 i2 p1 p2
